lean/FlowAnalysis/ValueVersion/Basic.lean
@@ -1,0 +1,41 @@
+module
+
+namespace FlowAnalysis
+
+-- TODO: this is a placeholder.
+public structure ValueVersion where
+
+namespace ValueVersion
+
+public def join (version₁? version₂? : Option ValueVersion) : Option ValueVersion :=
+  match version₁?, version₂? with
+    | none, none => none
+    | _,    _    => some ⟨⟩
+
+/-- The join operation is idempotent (`join version? version? = version?`). -/
+@[simp]
+public theorem join_self (version? : Option ValueVersion) : join version? version? = version? := by
+  cases version? <;> rfl
+
+public instance join.instIdempotentOp : Std.IdempotentOp join where
+  idempotent := join_self
+
+/-- The join operation is commutative (`join version?₁ version?₂ = join version?₂ version?₁`). -/
+public theorem join_comm (version?₁ version?₂ : Option ValueVersion) : join version?₁ version?₂ = join version?₂ version?₁ := by
+  cases version?₁ <;> cases version?₂ <;> rfl
+
+public instance join.instCommutative : Std.Commutative join where
+  comm := join_comm
+
+/--
+The join operation is associative (`join (join version?₁ version?₂) version?₃ = join version?₁ (join version?₂ version?₃)`).
+-/
+public theorem join_assoc (version?₁ version?₂ version?₃ : Option ValueVersion) :
+    join (join version?₁ version?₂) version?₃ = join version?₁ (join version?₂ version?₃) := by
+  cases version?₁ <;> cases version?₂ <;> cases version?₃ <;> rfl
+
+public instance join.instAssociative : Std.Associative join where
+  assoc := join_assoc
+
+end ValueVersion
+end FlowAnalysis
